

**Formatting:** Start a new page for each problem.

**1. (16 pts.) Asymptotic Growth**

In each of the following situations, indicate whether  $f(n) = O(g)$ ,  $f(n) = \Omega(g)$ , or  $f(n) = \Theta(g)$ .

- $f(n) = n^3 + n^2$ ,  $g(n) = n^3$
- $f(n) = n \log n$ ,  $g(n) = (\log n)^3$
- $f(n) = 2^n$ ,  $g(n) = 2^{n-1}$
- $f(n) = n^3 2^n$ ,  $g(n) = 3^n$
- $f(n) = \sqrt{n}$ ,  $g(n) = \log n$
- $f(n) = \log(n!)$ ,  $g(n) = n \log n$
- $f(n) = n!$ ,  $g(n) = 2^n \cdot n^2$
- $f(n) = n^{\log \log n}$ ,  $g(n) = \log(n^{\log n})$

**Answer:**

- $f(n) = \Theta(g)$   
**Explanation:**  $\lim_{n \rightarrow \infty} \frac{f(n)}{g(n)} = \lim_{n \rightarrow \infty} \frac{n^3 + n^2}{n^3} = \lim_{n \rightarrow \infty} (1 + \frac{1}{n}) = 1$

- $f(n) = \Omega(g)$   
**Explanation:**  $g(n) = (\log n)^2 \log n$ ,  $n$  grows faster than  $(\log n)^2$

- $f(n) = \Theta(g)$   
**Explanation:**  $\lim_{n \rightarrow \infty} \frac{f(n)}{g(n)} = \lim_{n \rightarrow \infty} \frac{2^n}{2^{n-1}} = 2$

- $f(n) = O(g)$   
**Explanation:**  $\lim_{n \rightarrow \infty} \frac{f(n)}{g(n)} = \lim_{n \rightarrow \infty} \frac{n^3 2^n}{3^n} = \lim_{n \rightarrow \infty} n^3 (\frac{2}{3})^n = 0$

- $f(n) = \Omega(g)$

- $f(n) = \Theta(g)$

**Explanation 1:** The proof is similar to how we proved problem 2.1 in recitation 1. We know  $\log(n!) = \sum_{k=1}^n \log k = \log 1 + \log 2 + \dots + \log n$ .

Upper bound: Since  $k \leq n$ , every term in the sum is at most  $n$ , so

$$\log(n!) \leq \sum_{k=1}^n \log n = n \log n.$$

Lower bound: We only look at the second half of the sum. Each of these terms is at least  $\log \frac{n}{2}$ , and there are  $\frac{n}{2}$  such terms (assuming without loss of generality that  $n$  is even). Therefore:

$$\log(n!) \geq \frac{n}{2} \log \frac{n}{2} = \frac{n}{2} (\log n - \log 2) = \frac{1}{2} n \log n - \frac{\log 2}{2} n.$$

**Explanation 2:** If you're familiar with Stirling's approximation, you can also prove it more easily by computing the limit:

$$\lim_{n \rightarrow \infty} \frac{f(n)}{g(n)} = \lim_{n \rightarrow \infty} \frac{\log(n!)}{n \log n} \approx \lim_{n \rightarrow \infty} \frac{n \log n - n}{n \log n} = \lim_{n \rightarrow \infty} \left(1 - \frac{1}{\log n}\right) = 1$$

- $f(n) = \Omega(g)$ ,

**Explanation:**  $f(n) = n(n-1)(n-2)! = O(n^2 n!)$ ,  $n^2$  grows slower than  $2^n$ , thus  $f(n) = \Omega(g)$

- $f(n) = \Omega(g)$

**Explanation:** Recall the logarithm theorem  $a^{\log_b c} = c^{\log_b a}$  and  $\log_b a^c = c \log_b a$ , and thus we have:

$$\lim_{n \rightarrow \infty} \frac{f(n)}{g(n)} = \lim_{n \rightarrow \infty} \frac{(\log n)^{\log n}}{(\log n)^2} = \lim_{n \rightarrow \infty} (\log n)^{(\log n - 2)} = \infty$$

**2. (17 pts.)** Let  $f, g$  be any functions from  $\mathbb{N}$  to  $(0, \infty)$ . Then prove or disprove the following:

- (3 pts)  $f = o(g) \Rightarrow f = O(g)$
- (3 pts)  $f = O(g) \vee f = \Omega(g)$
- (3 pts)  $f = O(g) \wedge f \neq \Theta(g) \Rightarrow f = o(g)$
- (4 pts) Let  $\mathcal{F}$  denote the set of all functions from  $\mathbb{N}$  to  $(0, \infty)$ . Then  $\Theta$  defines an equivalence relation on  $\mathcal{F}$ . (A relation  $\mathcal{R}$  on a set  $S$  is an equivalence relation if it is reflexive, symmetric and transitive.)
- (4 pts) For any increasing sublinear function  $t : (0, \infty) \rightarrow (0, \infty)$ ,  $f = O(g) \Rightarrow t \circ f = O(t \circ g)$ . We define  $t$  is *sublinear* if for all  $\alpha > 0$ ,  $x > 0$ , we have  $t(\alpha x) \leq \alpha t(x)$ . Also,  $t \circ f$  is a function defined as  $(t \circ f)(n) = t(f(n))$ .

**Answer:**

- True. *Proof.* Since  $f = o(g)$ , by the definition of small-o, we know that for every  $c > 0$ , there exists integer  $M_c \geq 0$  such that  $f(n) \leq c \cdot g(n)$  when  $n \geq M_c$ . Pick  $c = 1$ . Then there must exist integer  $M \geq 0$  such that  $f(n) \leq g(n)$  when  $n \geq M$ . This shows that  $f = O(g)$ , by the definition of big-O.
- False. Consider counter-example where  $f(n) = n$  and  $g(n) := \begin{cases} n^2, & n \text{ is even} \\ 1, & n \text{ is odd} \end{cases}$ . We first prove  $f \neq O(g)$ . This is because there does not exist  $c > 0$  and  $N \geq 0$  such that  $f(n) \leq c \cdot g(n)$  when  $n \geq N$ . To see it, note that  $n$  can be an arbitrarily large odd number, and for such odd  $n$ , we have  $f(n) = n$  and  $g(n) = 1$  and it is not possible to have  $f(n) = n \leq c \cdot g(n) = c$  since  $c$  is a constant and  $n$  can be arbitrarily large. Similarly, we can show  $f \neq \Omega(g)$ , i.e., there does not exist  $c > 0$  and  $N \geq 0$  such that  $f(n) \geq c \cdot g(n)$  when  $n \geq N$ . This is because  $n$  can be an arbitrarily large even number, and for such even  $n$ , we have  $f(n) = n$  and  $g(n) = n^2$  and it is not possible to have  $f(n) = n \geq c \cdot g(n) = c \cdot n^2$  since  $c$  is a constant and  $n$  can be arbitrarily large.
- False. Counter-example:  $f(n) := \begin{cases} n, & n \text{ is even} \\ 1, & n \text{ is odd} \end{cases}$  and  $g(n) = n$ . Clearly,  $f = O(g)$  because  $f(n) \leq g(n)$ . It is also obvious that  $f \neq \Omega(g)$  using a similar argument in above part. (Details:  $n$  can be an arbitrarily large odd integer, and for such  $n$  we have  $f(n) = 1$  and hence not possible to have  $f(n) = 1 \geq c \cdot f(n) = c \cdot n$  since  $c$  is a constant while  $n$  can be arbitrarily large.) Combined,  $f \neq \Theta(g)$ . But,  $f \neq o(g)$ . This is because, for any  $0 < c < 1$  we cannot find  $N_c \geq 0$  such that  $f(n) \leq c \cdot g(n)$ , since we can always find an arbitrarily large even  $n$  and for such  $n$  we have  $f(n) = n > c \cdot g(n) = c \cdot n$  as  $c < 1$ .

- **True. Proof.** We show reflexivity, symmetry, and transitivity for  $\Theta$ .
  - **Reflexivity:** We need to show that every function is  $\Theta$ -related to itself. For any function  $f \in \mathcal{F}$ , since  $f(n) = f(n)$  for all  $n$ , it follows that  $f = O(g)$  and  $f = \Omega(n)$  and hence  $f = \Theta(f)$ .
  - **Symmetry:** We need to show that if  $f = \Theta(g)$ , then  $g = \Theta(f)$ . By the definition of  $\Theta$ , if  $f = \Theta(g)$ , then we have  $f = O(g)$  and  $f = \Omega(g)$ .  $f = O(g)$  implies  $g = \Omega(f)$ , and  $f = \Omega(g)$  implies  $g = O(f)$ . Combining  $g = \Omega(f)$  and  $g = O(f)$  we get  $g = \Theta(f)$ .
  - **Transitivity:** We need to show that if  $f = \Theta(g)$  and  $g = \Theta(h)$ , then  $f = \Theta(h)$ .  
 We know that  $f = \Theta(g)$  and  $g = \Theta(h)$  imply  $f = O(g)$  and  $g = O(h)$ ; we first use these two to derive that  $f = O(h)$ . By definition of big-O, there exists  $c_1 > 0$  and  $N_1 \geq 0$  such that  $f(n) \leq c_1 \cdot g(n)$  when  $n \geq N_1$ , and there exists  $c_2 > 0$  and  $N_2 \geq 0$  such that  $g(n) \leq c_2 \cdot h(n)$  when  $n \geq N_2$ . Let  $c = c_1 \cdot c_2$  and  $N = \max\{N_1, N_2\}$ . Therefore, when  $n \geq N$ , we must have  $f(n) \leq c_1 \cdot g(n) \leq c_1 \cdot c_2 \cdot h(n) = c \cdot g(n)$ . This proves that  $f = O(h)$ .  
 We also know that  $f = \Theta(g)$  and  $g = \Theta(h)$  imply  $f = \Omega(g)$  and  $g = \Omega(h)$ . We can use these two to derive that  $f = \Omega(h)$  in a similar way. By definition of big-Omega, there exists  $c_1 > 0$  and  $N_1 \geq 0$  such that  $f(n) \geq c_1 \cdot g(n)$  when  $n \geq N_1$ , and there exists  $c_2 > 0$  and  $N_2 \geq 0$  such that  $g(n) \geq c_2 \cdot h(n)$  when  $n \geq N_2$ . Let  $c = c_1 \cdot c_2$  and  $N = \max\{N_1, N_2\}$ . Therefore, when  $n \geq N$ , we must have  $f(n) \geq c_1 \cdot g(n) \geq c_1 \cdot c_2 \cdot h(n) = c \cdot g(n)$ . This proves that  $f = \Omega(h)$ .
- **True. Proof.**  $f = O(g)$  implies there exists some  $N \geq 0$  and  $c > 0$  s.t.  $f(n) \leq c \cdot g(n)$  for all  $n \geq N$ . For the same  $c$  and  $N$ , since  $t$  is increasing, we have  $t \circ f(n) = t(f(n)) \leq t(c \cdot g(n))$ . By further using the sublinearity property of  $t$ , we get  $t(c \cdot g(n)) \leq c \cdot t(g(n)) = c \cdot t \circ g(n)$ . Combined, for the same  $c$  and  $N$ , we have  $t \circ f(n) \leq c \cdot t \circ g(n)$  for all  $n \geq N$ . By definition, this proves  $t \circ f = O(t \circ g)$ .

**3. (15 + 5 (bonus) pts.)** For each pseudo-code below, give the asymptotic running time in  $\Theta$  notation. You may assume that standard arithmetic operations take  $\Theta(1)$  time. (The 4th one is a bonus problem.)

---

```

k := 0;
for i := 1 to n do
1.   for j := i to n do
      |   k := k + 1;
      end
    end

```

---

**Explanation:**

The outer loop runs for  $i = 1$  to  $n$ . For a given  $i$ , the inner loop runs for  $j$  from  $i$  to  $n$ , and for each  $j$  it takes  $\Theta(1)$  time to do the “ $k := k + 1$ ”. The total running time is therefore:

$$\sum_{i=1}^n \sum_{j=i}^n 1 = \sum_{i=1}^n (n - i + 1) = \sum_{i=1}^n (n + 1 - i) = (n + 1) \cdot n - \sum_{i=1}^n i = \frac{n(n + 1)}{2}$$

**Answer:** Therefore, the running time is  $\Theta(n^2)$ .

---



---

```

2.  for  $i := 1$  to  $n$  do
    |   for  $j := 1$  to  $n$  do
    |   |    $k := j$ ;
    |   |   while  $k \geq 1$  do
    |   |   |    $k := k - 1$ ;
    |   |   end
    |   end
    end
end

```

---

**Explanation:**

- The outer ‘for’ loop runs from  $i = 1$  to  $n$ , thus executing  $n$  times.
- The inner ‘for’ loop also runs from  $j = 1$  to  $n$ , meaning it also executes  $n$  times.
- Inside the inner loop, there’s a ‘while’ loop that runs while  $k \geq 1$ , where  $k$  starts as  $j$  and decrements by 1 until  $k = 0$ . This means the ‘while’ loop runs  $j$  times for each value of  $j$ .

Hence, the total running time of the algorithm is:

$$T(n) = \sum_{i=1}^n \sum_{j=1}^n j = \sum_{i=1}^n \frac{n(n+1)}{2} = \frac{n^3 + n^2}{2}$$

**Answer:** Therefore, the total running time is  $\Theta(n^3)$ .

---



---

```

3.  for  $i := 1$  to  $n$  do
    |    $j := 1$ ;
    |   while  $j \leq n$  do
    |   |    $j := j \times 2$ ;
    |   end
    end
end

```

---

**Explanation:**

- The outer ‘for’ loop runs from  $i = 1$  to  $n$ , so it executes  $n$  times.
- Inside the outer loop, the ‘while’ loop starts with  $j = 1$  and keeps doubling  $j$  until  $j > n$ . This means the number of iterations of the ‘while’ loop is proportional to the number of times  $j$  can be doubled before it exceeds  $n$ .

The value of  $j$  increases as  $1, 2, 4, 8, \dots$ , up to  $2^k \leq n$ . The number of iterations is therefore  $\log_2(n)$ .

Thus, the ‘while’ loop runs  $\Theta(\log n)$  times for each iteration of the outer ‘for’ loop.

**Answer:** Since the outer loop runs  $n$  times, the total running time of the algorithm is:

$$T(n) = n \times \Theta(\log n) = \Theta(n \log n)$$


---



---

```

4.  for  $i := 1$  to  $n$  do
    |    $j := i$ ;
    |   while  $j \leq n$  do
    |   |    $j := j + i$ ;
    |   end
    end
end

```

---

**Explanation:**

- The outer ‘for’ loop runs from  $i = 1$  to  $n$ , meaning it executes  $n$  times.
- Inside the outer loop, the ‘while’ loop starts with  $j = i$  and increments  $j$  by  $i$  in each iteration until  $j > n$ .

For a given  $i$ , the number of iterations of the ‘while’ loop is the number of steps it takes to go from  $i$  to  $n$  by increments of  $i$ . This is approximately  $\frac{n}{i}$ .

Thus, the total number of iterations of the ‘while’ loop over all values of  $i$  is:

$$\sum_{i=1}^n \frac{n}{i}$$

This is  $n$  times the harmonic series:

$$n \times H_n = n \times (\log n + O(1))$$

**Answer:** Therefore, the total running time is  $\Theta(n \log n)$ .

#### 4. (15 pts.) Master’s Theorem

Solve each of the following recurrences. Give the closed form of  $T(n)$  in  $\Theta$ -notation. You may assume that  $n$  is of a special form (e.g., a power of two or another number) and that the recurrence has a convenient base case that is  $\Theta(1)$ .

- (3 pts)  $T(n) = 4 \cdot T(n/4) + n$
- (3 pts)  $T(n) = 6 \cdot T(n/3) + n^2$
- (3 pts)  $T(n) = 4 \cdot T(n/8) + \log n$
- (3 pts)  $T(n) = 2 \cdot T(n/2) + n \log n$
- (3 pts)  $T(n) = 8 \cdot T(n/3) + 2^n$

**Answer:**

- $T(n) = \Theta(n \log n)$

**Explanation:** Apply the Master’s theorem, where  $a = 4, b = 4, d = 1$ . We have  $d = \log_b a$ . Hence, we apply Case 1, leading to  $T(n) = \Theta(n^d) = \Theta(n \log n)$ .

- $T(n) = \Theta(n^2)$

**Explanation:** We have  $a = 6, b = 3, d = 2$ , which means  $d > \log_b a = \log_3 6$ . Hence, we apply Case 2, leading to  $T(n) = \Theta(n^2)$ .

- $T(n) = \Theta(n^{2/3})$

**Explanation:** We have  $a = 4, b = 8, d = 0$ , which means  $d < \log_b a = \log_8 4 = 2/3$ . Hence, we apply Case 2, leading to  $T(n) = \Theta(n^{2/3})$ .

- $T(n) = \Theta(n \log^2 n)$

**Explanation:** We have  $a = 2, b = 2, d = 1$ , which means  $d = \log_b a$ . Hence, we apply Case 1, leading to  $T(n) = \Theta(n \log^2 n)$ .

- $T(n) = \Theta(2^n)$

**Explanation:** The running time of the merging step takes  $\Theta(2^n)$ , which grows faster than any polynomial-time function. This makes us guess that the running time is dominated by  $\Theta(2^n)$ . We now prove it.

Note that  $T(n) = 8 \cdot T(n/3) + 2^n \geq 2^n$ . Hence  $T(n) = \Omega(2^n)$ . We therefore just need to prove  $T(n) = O(2^n)$ . By definition, that requires to show the existence of  $c > 0$  and  $N \geq 0$  such that  $T(n) \leq c \cdot 2^n$  when  $n \geq N$ . Without loss of generality, we assume that  $n$  is a power of 3, that is, we assume there exists  $k$  such that  $n = 3^k$ . Now we need to prove there exists  $c > 0$  and  $K \geq 0$  such that  $T(3^k) \leq c \cdot 2^{3^k}$  when  $k \geq K$ .

We prove above by induction. We choose  $c = 2$  and  $K = 1$ . The base case is  $k = 1$ , i.e.,  $n = 3^k = 3$ . It is easy to verify that  $T(n) = T(3) = 8 \cdot T(1) + 2^3 = 8 + 8 = 16$ , while  $c \cdot 2^{3^k} = 2 \cdot 2^3 = 16$ . So, the base case holds.

For the inductive step, assume that  $T(3^k) \leq c \cdot 2^{3^k}$  holds up to  $n = 3^k$ . Now we prove it for  $n = 3^{k+1}$ . We can write:

$$\begin{aligned} T(3^{k+1}) &= 8 \cdot T(3^{k+1}/3) + 2^{3^{k+1}} \\ &= 8 \cdot T(3^k) + 2^{3^{k+1}} \\ &\leq 8 \cdot c \cdot 2^{3^k} + 2^{3^{k+1}} \\ &= 16 \cdot 2^{3^k} + 2^{3^{k+1}} \\ &= 2^{3^k+4} + 2^{3^{k+1}} \\ &\leq 2 \cdot 2^{3^{k+1}} \end{aligned}$$

The last inequality holds because  $3^k + 4 \leq 3^{k+1}$  when  $k \geq 1$ .

# Rubric:

## Problem 1, 16 pts

2 points for each correct solution

## Problem 2, 17 pts

- Parts (i), (ii), (iii) and (v) - Full credit if correct proof shown. Partial credit (1 pt) if incorrect proof, but correct option out of T and F mentioned; zero otherwise.
- Part (iv) - Full credit if correct proof shown for all 3 cases shown. Partial credit is: +1 for correct proof of reflexivity, +1 for correct proof of symmetry and +1 for correct proof of transitivity.

## Problem 3, 15 + 5 (Bonus) pts

For each part:

- full credit (+5) for correct solution with proper justification.
- partial credit (+3) for right answer with no or incorrect justification.
- partial credit (+4) for right answer with partially correct justification.

## Problem 4, 15 pts

For each part:

- full credit (+3) for correct solution with proper justification.
- partial credit (+2) for right answer with no, or incorrect justification.